<?xml version="1.0"?>
<rdf:RDF xmlns="http://w3id.org/rml/lv/"
     xml:base="http://w3id.org/rml/lv/"
     xmlns:ns="http://creativecommons.org/ns#"
     xmlns:owl="http://www.w3.org/2002/07/owl#"
     xmlns:rdf="http://www.w3.org/1999/02/22-rdf-syntax-ns#"
     xmlns:rml="http://w3id.org/rml/"
     xmlns:xml="http://www.w3.org/XML/1998/namespace"
     xmlns:xsd="http://www.w3.org/2001/XMLSchema#"
     xmlns:bibo="http://purl.org/ontology/bibo/"
     xmlns:foaf="http://xmlns.com/foaf/0.1/"
     xmlns:rdfs="http://www.w3.org/2000/01/rdf-schema#"
     xmlns:vaem="http://www.linkedmodel.org/schema/vaem#"
     xmlns:vann="http://purl.org/vocab/vann/"
     xmlns:shacl="http://www.w3.org/ns/shacl#"
     xmlns:terms="http://purl.org/dc/terms/">
    <owl:Ontology rdf:about="http://w3id.org/rml/lv/">
        <owl:versionIRI rdf:resource="http://w3id.org/rml/lv/"/>
        <owl:imports rdf:resource="https://kg-construct.github.io/rml-core/ontology/documentation/ontology.ttl"/>
        <owl:imports rdf:resource="https://kg-construct.github.io/rml-io/ontology/documentation/ontology.ttl"/>
        <terms:contributor>Ana Iglesias Molina</terms:contributor>
        <terms:contributor>Ben De Meester</terms:contributor>
        <terms:contributor>Davide Lanti</terms:contributor>
        <terms:contributor>Els de Vleeschauwer</terms:contributor>
        <terms:contributor>Pano Maria</terms:contributor>
        <terms:contributor>Thomas Delva</terms:contributor>
        <terms:created>2024-01-01</terms:created>
        <terms:description xml:lang="en">RML Logical Views flatten nested data, allow flexible joining of data sources, and handle mix source formats.</terms:description>
        <terms:license rdf:resource="http://purl.org/NET/rdflicense/cc-by4.0"/>
        <terms:modified>2024-12-02</terms:modified>
        <terms:publisher rdf:resource="https://www.w3.org/community/kg-construct/"/>
        <terms:title xml:lang="en">RML Logical Views</terms:title>
        <bibo:status>draft</bibo:status>
        <vann:preferredNamespacePrefix>rml</vann:preferredNamespacePrefix>
        <vann:preferredNamespaceUri>http://w3id.org/rml/</vann:preferredNamespaceUri>
        <owl:versionInfo>0.1.0</owl:versionInfo>
        <shacl:suggestedShapesGraph rdf:resource="http://w3id.org/rml/lv/shapes"/>
    </owl:Ontology>
    


    <!-- 
    ///////////////////////////////////////////////////////////////////////////////////////
    //
    // Annotation properties
    //
    ///////////////////////////////////////////////////////////////////////////////////////
     -->


    


    <!-- http://www.w3.org/ns/shacl#suggestedShapesGraph -->


    <owl:AnnotationProperty rdf:about="http://www.w3.org/ns/shacl#suggestedShapesGraph"/>
    


    <!-- 
    ///////////////////////////////////////////////////////////////////////////////////////
    //
    // Object Properties
    //
    ///////////////////////////////////////////////////////////////////////////////////////
     -->


    


    <!-- http://w3id.org/rml/field -->


    <owl:ObjectProperty rdf:about="http://w3id.org/rml/field">
        <rdfs:domain>
            <owl:Class>
                <owl:unionOf rdf:parseType="Collection">
                    <rdf:Description rdf:about="http://w3id.org/rml/Field"/>
                    <rdf:Description rdf:about="http://w3id.org/rml/LogicalView"/>
                </owl:unionOf>
            </owl:Class>
        </rdfs:domain>
        <rdfs:range rdf:resource="http://w3id.org/rml/Field"/>
        <rdfs:comment>A field of the logical view.</rdfs:comment>
        <rdfs:isDefinedBy rdf:resource="http://w3id.org/rml/lv/"/>
        <rdfs:label>field</rdfs:label>
    </owl:ObjectProperty>
    


    <!-- http://w3id.org/rml/innerJoin -->


    <owl:ObjectProperty rdf:about="http://w3id.org/rml/innerJoin">
        <rdfs:domain rdf:resource="http://w3id.org/rml/LogicalView"/>
        <rdfs:range rdf:resource="http://w3id.org/rml/LogicalViewJoin"/>
        <rdfs:comment>An inner join of the logical view.</rdfs:comment>
        <rdfs:isDefinedBy rdf:resource="http://w3id.org/rml/lv/"/>
        <rdfs:label>inner join</rdfs:label>
    </owl:ObjectProperty>
    


    <!-- http://w3id.org/rml/leftJoin -->


    <owl:ObjectProperty rdf:about="http://w3id.org/rml/leftJoin">
        <rdfs:domain rdf:resource="http://w3id.org/rml/LogicalView"/>
        <rdfs:range rdf:resource="http://w3id.org/rml/LogicalViewJoin"/>
        <rdfs:comment>A left join of the logical view.</rdfs:comment>
        <rdfs:isDefinedBy rdf:resource="http://w3id.org/rml/lv/"/>
        <rdfs:label>left join</rdfs:label>
    </owl:ObjectProperty>
    


    <!-- http://w3id.org/rml/onFields -->


    <owl:ObjectProperty rdf:about="http://w3id.org/rml/onFields">
        <rdfs:domain rdf:resource="http://w3id.org/rml/StructuralAnnotation"/>
        <rdfs:range rdf:resource="http://www.w3.org/1999/02/22-rdf-syntax-ns#List"/>
        <rdfs:comment>
          The property onFields specifies the fields in LogicalView that are involved by the structural annotation.
          The semantics of this involvement depends on the specific annotation.
          </rdfs:comment>
        <rdfs:isDefinedBy rdf:resource="http://w3id.org/rml/lv/"/>
        <rdfs:label>on fields</rdfs:label>
    </owl:ObjectProperty>
    


    <!-- http://w3id.org/rml/parentLogicalView -->


    <owl:ObjectProperty rdf:about="http://w3id.org/rml/parentLogicalView">
        <rdfs:domain rdf:resource="http://w3id.org/rml/LogicalViewJoin"/>
        <rdfs:range rdf:resource="http://w3id.org/rml/LogicalView"/>
        <rdfs:comment>The parent logical view of the logical view join.</rdfs:comment>
        <rdfs:isDefinedBy rdf:resource="http://w3id.org/rml/lv/"/>
        <rdfs:label>parent logical view</rdfs:label>
    </owl:ObjectProperty>
    


    <!-- http://w3id.org/rml/structuralAnnotation -->


    <owl:ObjectProperty rdf:about="http://w3id.org/rml/structuralAnnotation">
        <rdfs:domain rdf:resource="http://w3id.org/rml/LogicalView"/>
        <rdfs:range rdf:resource="http://w3id.org/rml/StructuralAnnotation"/>
        <rdfs:comment>A structural annotation of the logical view.</rdfs:comment>
        <rdfs:isDefinedBy rdf:resource="http://w3id.org/rml/lv/"/>
        <rdfs:label>structural annotation</rdfs:label>
    </owl:ObjectProperty>
    


    <!-- http://w3id.org/rml/targetFields -->


    <owl:ObjectProperty rdf:about="http://w3id.org/rml/targetFields">
        <rdfs:domain rdf:resource="http://w3id.org/rml/StructuralAnnotation"/>
        <rdfs:range rdf:resource="http://www.w3.org/1999/02/22-rdf-syntax-ns#List"/>
        <rdfs:comment>The property targetFields specifies the Fields target of the InclusionAnnotation.</rdfs:comment>
        <rdfs:isDefinedBy rdf:resource="http://w3id.org/rml/lv/"/>
        <rdfs:label>target fields</rdfs:label>
    </owl:ObjectProperty>
    


    <!-- http://w3id.org/rml/targetView -->


    <owl:ObjectProperty rdf:about="http://w3id.org/rml/targetView">
        <rdfs:domain rdf:resource="http://w3id.org/rml/InclusionDependencyAnnotation"/>
        <rdfs:range rdf:resource="http://w3id.org/rml/LogicalView"/>
        <rdfs:comment>The property targetFields specifies the Fields target of the InclusionAnnotation.</rdfs:comment>
        <rdfs:isDefinedBy rdf:resource="http://w3id.org/rml/lv/"/>
        <rdfs:label>target view</rdfs:label>
    </owl:ObjectProperty>
    


    <!-- http://w3id.org/rml/viewOn -->


    <owl:ObjectProperty rdf:about="http://w3id.org/rml/viewOn">
        <rdfs:domain rdf:resource="http://w3id.org/rml/LogicalView"/>
        <rdfs:range rdf:resource="http://w3id.org/rml/AbstractLogicalSource"/>
        <rdfs:comment>The source of the logical view. This is the abstract logical source from which the logical view is derived.</rdfs:comment>
        <rdfs:isDefinedBy rdf:resource="http://w3id.org/rml/lv/"/>
        <rdfs:label>view on</rdfs:label>
    </owl:ObjectProperty>
    


    <!-- 
    ///////////////////////////////////////////////////////////////////////////////////////
    //
    // Data properties
    //
    ///////////////////////////////////////////////////////////////////////////////////////
     -->


    


    <!-- http://w3id.org/rml/fieldName -->


    <owl:DatatypeProperty rdf:about="http://w3id.org/rml/fieldName">
        <rdfs:domain rdf:resource="http://w3id.org/rml/Field"/>
        <rdfs:range rdf:resource="http://www.w3.org/2001/XMLSchema#string"/>
        <rdfs:comment>The name of the field.</rdfs:comment>
        <rdfs:isDefinedBy rdf:resource="http://w3id.org/rml/lv/"/>
        <rdfs:label>field name</rdfs:label>
    </owl:DatatypeProperty>
    


    <!-- 
    ///////////////////////////////////////////////////////////////////////////////////////
    //
    // Classes
    //
    ///////////////////////////////////////////////////////////////////////////////////////
     -->


    


    <!-- http://w3id.org/rml/AbstractLogicalSource -->


    <owl:Class rdf:about="http://w3id.org/rml/AbstractLogicalSource"/>
    


    <!-- http://w3id.org/rml/ExpressionField -->


    <owl:Class rdf:about="http://w3id.org/rml/ExpressionField">
        <rdfs:subClassOf rdf:resource="http://w3id.org/rml/ExpressionMap"/>
        <rdfs:subClassOf rdf:resource="http://w3id.org/rml/Field"/>
        <rdfs:comment>A expression field is an expression map that gives a name to an expression.</rdfs:comment>
        <rdfs:isDefinedBy rdf:resource="http://w3id.org/rml/lv/"/>
        <rdfs:label>Expression Field</rdfs:label>
    </owl:Class>
    


    <!-- http://w3id.org/rml/Field -->


    <owl:Class rdf:about="http://w3id.org/rml/Field">
        <rdfs:comment>A field gives a name to data derived from the abstract logical source on which a logical view is defined.</rdfs:comment>
        <rdfs:isDefinedBy rdf:resource="http://w3id.org/rml/lv/"/>
        <rdfs:label>Field</rdfs:label>
    </owl:Class>
    


    <!-- http://w3id.org/rml/ForeignKeyAnnotation -->


    <owl:Class rdf:about="http://w3id.org/rml/ForeignKeyAnnotation">
        <rdfs:subClassOf rdf:resource="http://w3id.org/rml/InclusionDependencyAnnotation"/>
        <rdfs:comment>A foreign key annotation is analogous to the notion of foreign key constraint in databases.</rdfs:comment>
        <rdfs:isDefinedBy rdf:resource="http://w3id.org/rml/lv/"/>
        <rdfs:label>Foreign Key Annotation</rdfs:label>
    </owl:Class>
    


    <!-- http://w3id.org/rml/IRISafeAnnotation -->


    <owl:Class rdf:about="http://w3id.org/rml/IRISafeAnnotation">
        <rdfs:subClassOf rdf:resource="http://w3id.org/rml/StructuralAnnotation"/>
        <rdfs:comment>A IRI safe annotation indicates that the field content is IRI safe.</rdfs:comment>
        <rdfs:isDefinedBy rdf:resource="http://w3id.org/rml/lv/"/>
        <rdfs:label>IRI Safe Annotation</rdfs:label>
    </owl:Class>
    


    <!-- http://w3id.org/rml/InclusionDependencyAnnotation -->


    <owl:Class rdf:about="http://w3id.org/rml/InclusionDependencyAnnotation">
        <rdfs:subClassOf rdf:resource="http://w3id.org/rml/StructuralAnnotation"/>
        <rdfs:comment>An inclusion dependency annotation is analogous to the notion of inclusion dependency in databases.</rdfs:comment>
        <rdfs:isDefinedBy rdf:resource="http://w3id.org/rml/lv/"/>
        <rdfs:label>Inclusion Dependency Annotation</rdfs:label>
    </owl:Class>
    


    <!-- http://w3id.org/rml/Iterable -->


    <owl:Class rdf:about="http://w3id.org/rml/Iterable"/>
    


    <!-- http://w3id.org/rml/IterableField -->


    <owl:Class rdf:about="http://w3id.org/rml/IterableField">
        <rdfs:subClassOf rdf:resource="http://w3id.org/rml/Field"/>
        <rdfs:subClassOf rdf:resource="http://w3id.org/rml/Iterable"/>
        <rdfs:comment>A iterable field is an iterable that gives a name to a logical iteration.</rdfs:comment>
        <rdfs:isDefinedBy rdf:resource="http://w3id.org/rml/lv/"/>
        <rdfs:label>Iterable Field</rdfs:label>
    </owl:Class>
    


    <!-- http://w3id.org/rml/LogicalView -->


    <owl:Class rdf:about="http://w3id.org/rml/LogicalView">
        <rdfs:subClassOf rdf:resource="http://w3id.org/rml/AbstractLogicalSource"/>
        <rdfs:comment>A logical view (rml:LogicalView) is a type of abstract logical source that is derived from another abstract logical source by defining field with data from said abstract logical source.</rdfs:comment>
        <rdfs:isDefinedBy rdf:resource="http://w3id.org/rml/lv/"/>
        <rdfs:label>Logical View</rdfs:label>
    </owl:Class>
    


    <!-- http://w3id.org/rml/LogicalViewJoin -->


    <owl:Class rdf:about="http://w3id.org/rml/LogicalViewJoin">
        <rdfs:comment>A logical view join is an operation that adapts the logical iterations of one logical view (the child logical view) with fields from another logical view (the parent logical view).</rdfs:comment>
        <rdfs:isDefinedBy rdf:resource="http://w3id.org/rml/lv/"/>
        <rdfs:label>Logical View Join</rdfs:label>
    </owl:Class>
    


    <!-- http://w3id.org/rml/NonNullableAnnotation -->


    <owl:Class rdf:about="http://w3id.org/rml/NonNullableAnnotation">
        <rdfs:subClassOf rdf:resource="http://w3id.org/rml/StructuralAnnotation"/>
        <rdfs:comment>A non nullable annotation is analogous to the notion of NOT NULL constraints in databases.</rdfs:comment>
        <rdfs:isDefinedBy rdf:resource="http://w3id.org/rml/lv/"/>
        <rdfs:label>Non Nullable Annotation</rdfs:label>
    </owl:Class>
    


    <!-- http://w3id.org/rml/PrimaryKeyAnnotation -->


    <owl:Class rdf:about="http://w3id.org/rml/PrimaryKeyAnnotation">
        <rdfs:subClassOf rdf:resource="http://w3id.org/rml/NonNullableAnnotation"/>
        <rdfs:subClassOf rdf:resource="http://w3id.org/rml/UniqueAnnotation"/>
        <rdfs:comment>A primary key annotation is analogous to the notion of a primary key constraints in databases.</rdfs:comment>
        <rdfs:isDefinedBy rdf:resource="http://w3id.org/rml/lv/"/>
        <rdfs:label>Primary Key Annotation</rdfs:label>
    </owl:Class>
    


    <!-- http://w3id.org/rml/StructuralAnnotation -->


    <owl:Class rdf:about="http://w3id.org/rml/StructuralAnnotation">
        <rdfs:comment>A structural annotation provide a mechanism to express relationships between logical views, as well as additional information about fields.</rdfs:comment>
        <rdfs:isDefinedBy rdf:resource="http://w3id.org/rml/lv/"/>
        <rdfs:label>Structural Annotation</rdfs:label>
    </owl:Class>
    


    <!-- http://w3id.org/rml/UniqueAnnotation -->


    <owl:Class rdf:about="http://w3id.org/rml/UniqueAnnotation">
        <rdfs:subClassOf rdf:resource="http://w3id.org/rml/StructuralAnnotation"/>
        <rdfs:comment>A unique annotation is analogous to the notion of UNIQUE constraints in databases. .</rdfs:comment>
        <rdfs:isDefinedBy rdf:resource="http://w3id.org/rml/lv/"/>
        <rdfs:label>Unique Annotation</rdfs:label>
    </owl:Class>
    


    <!-- http://www.w3.org/1999/02/22-rdf-syntax-ns#List -->


    <owl:Class rdf:about="http://www.w3.org/1999/02/22-rdf-syntax-ns#List"/>
</rdf:RDF>



<!-- Generated by the OWL API (version 5.1.18) https://github.com/owlcs/owlapi/ -->


