@prefix : <http://w3id.org/rml/lv/> .
@prefix sh: <http://www.w3.org/ns/shacl#> .
@prefix owl: <http://www.w3.org/2002/07/owl#> .
@prefix rdf: <http://www.w3.org/1999/02/22-rdf-syntax-ns#> .
@prefix rml: <http://w3id.org/rml/> .
@prefix xml: <http://www.w3.org/XML/1998/namespace> .
@prefix xsd: <http://www.w3.org/2001/XMLSchema#> .
@prefix rdfs: <http://www.w3.org/2000/01/rdf-schema#> .
@prefix cc: <http://creativecommons.org/ns#> .
@prefix dc: <http://purl.org/dc/terms/> .
@prefix vann: <http://purl.org/vocab/vann/> .
@prefix bibo: <http://purl.org/ontology/bibo/> .
@base <http://w3id.org/rml/lv/> .


<http://w3id.org/rml/lv/> rdf:type owl:Ontology ;
                           owl:imports <https://kg-construct.github.io/rml-core/ontology/documentation/ontology.ttl> ,
                                       <https://kg-construct.github.io/rml-io/ontology/documentation/ontology.ttl> ;
                           sh:suggestedShapesGraph :shapes ;
                           dc:description "RML Logical Views flatten nested data, allow flexible joining of data sources, and handle mix source formats."@en ;
                           dc:title "RML Logical Views"@en ;
                           dc:contributor "Pano Maria" ;
                           dc:contributor "Els de Vleeschauwer" ;
                           dc:contributor "Davide Lanti" ;
                           dc:license <http://purl.org/NET/rdflicense/cc-by4.0> ;
                           vann:preferredNamespaceUri "http://w3id.org/rml/" ;
                           vann:preferredNamespacePrefix "rml" ;
                           dc:publisher <https://www.w3.org/community/kg-construct/> ;
                           bibo:status "draft" ;
                           owl:versionIRI <http://w3id.org/rml/lv/> ;
                           owl:versionInfo "0.1.0" ;
                           dc:created "2025-01-14" ;
                           dc:modified "2025-01-14" .

#################################################################
#    Annotation properties
#################################################################

###  http://www.w3.org/ns/shacl#suggestedShapesGraph
sh:suggestedShapesGraph rdf:type owl:AnnotationProperty .


#################################################################
#    Object Properties
#################################################################

###  http://w3id.org/rml/field
rml:field rdf:type owl:ObjectProperty ;
          rdfs:label "field" ;
          rdfs:comment "A field of the logical view." ;
          rdfs:domain [ owl:unionOf ( rml:LogicalView rml:Field )] ;
          rdfs:range rml:Field ;
          rdfs:isDefinedBy <http://w3id.org/rml/lv/> .


### http://w3id.org/rml/viewOn
rml:viewOn rdf:type owl:ObjectProperty ;
          rdfs:label "view on" ;
          rdfs:comment "The source of the logical view. This is the abstract logical source from which the logical view is derived." ;
          rdfs:domain rml:LogicalView ;
          rdfs:range rml:AbstractLogicalSource ;
          rdfs:isDefinedBy <http://w3id.org/rml/lv/> .


###  http://w3id.org/rml/innerJoin
rml:innerJoin rdf:type owl:ObjectProperty ;
              rdfs:label "inner join" ;
              rdfs:comment "An inner join of the logical view." ;
              rdfs:domain rml:LogicalView ;
              rdfs:range rml:LogicalViewJoin ;
              rdfs:isDefinedBy <http://w3id.org/rml/lv/> .


###  http://w3id.org/rml/leftJoin
rml:leftJoin rdf:type owl:ObjectProperty ;
             rdfs:label "left join" ;
             rdfs:comment "A left join of the logical view." ;
             rdfs:domain rml:LogicalView ;
             rdfs:range rml:LogicalViewJoin ;
             rdfs:isDefinedBy <http://w3id.org/rml/lv/> .


###  http://w3id.org/rml/parentLogicalView
rml:parentLogicalView rdf:type owl:ObjectProperty ;
                      rdfs:label "parent logical view" ;
                      rdfs:comment "The parent logical view of the logical view join." ;
                      rdfs:domain rml:LogicalViewJoin ;
                      rdfs:range rml:LogicalView ;
                      rdfs:isDefinedBy <http://w3id.org/rml/lv/> .


###  http://w3id.org/rml/onFields
rml:onFields rdf:type owl:ObjectProperty ;
          rdfs:label "on fields" ;
          rdfs:comment """
          The property onFields specifies the fields in LogicalView that are involved by the structural annotation.
          The semantics of this involvement depends on the specific annotation.
          """ ;
          rdfs:domain rml:StructuralAnnotation ;
          rdfs:range rdf:List ;
          rdfs:isDefinedBy <http://w3id.org/rml/lv/> .


###  http://w3id.org/rml/structuralAnnotation
rml:structuralAnnotation rdf:type owl:ObjectProperty ;
                      rdfs:label "structural annotation" ;
                      rdfs:comment "A structural annotation of the logical view." ;
                      rdfs:domain rml:LogicalView ;
                      rdfs:range rml:StructuralAnnotation ;
                      rdfs:isDefinedBy <http://w3id.org/rml/lv/> .

###  http://w3id.org/rml/targetFields
rml:targetFields rdf:type owl:ObjectProperty ;
              rdfs:label "target fields" ;
              rdfs:comment "The property targetFields specifies the Fields target of the InclusionAnnotation." ;
              rdfs:domain rml:StructuralAnnotation ;
              rdfs:range rdf:List ;
              rdfs:isDefinedBy <http://w3id.org/rml/lv/> .


###  http://w3id.org/rml/targetView
rml:targetView rdf:type owl:ObjectProperty ;
            rdfs:label "target view" ;
            rdfs:comment "The property targetFields specifies the Fields target of the InclusionAnnotation." ;
            rdfs:domain rml:InclusionDependencyAnnotation ;
            rdfs:range rml:LogicalView ;
            rdfs:isDefinedBy <http://w3id.org/rml/lv/> .


#################################################################
#    Data properties
#################################################################

###  http://w3id.org/rml/fieldName
rml:fieldName rdf:type owl:DatatypeProperty ;
              rdfs:label "field name" ;
              rdfs:comment "The name of the field." ;
              rdfs:domain rml:Field ;
              rdfs:range xsd:string ;
              rdfs:isDefinedBy <http://w3id.org/rml/lv/> .


#################################################################
#    Classes
#################################################################

###  http://w3id.org/rml/Field
rml:Field rdf:type owl:Class ;
          rdfs:label "Field" ;
          rdfs:comment "A field gives a name to data derived from the abstract logical source on which a logical view is defined." ;
          rdfs:isDefinedBy <http://w3id.org/rml/lv/> .

###  http://w3id.org/rml/ExpressionField
rml:ExpressionField rdf:type owl:Class ;
          rdfs:label "Expression Field" ;
          rdfs:comment "An expression field is an expression map that gives a name to an expression." ;
          rdfs:subClassOf rml:Field, rml:ExpressionMap ;
          rdfs:isDefinedBy <http://w3id.org/rml/lv/> .


###  http://w3id.org/rml/IterableField
rml:IterableField rdf:type owl:Class ;
          rdfs:label "Iterable Field" ;
          rdfs:comment "An iterable field is an iterable that gives a name to a logical iteration." ;
          rdfs:subClassOf rml:Field, rml:Iterable ;
          rdfs:isDefinedBy <http://w3id.org/rml/lv/> .


###  http://w3id.org/rml/LogicalView
rml:LogicalView rdf:type owl:Class ;
                rdfs:label "Logical View" ;
                rdfs:comment "A logical view (rml:LogicalView) is a type of abstract logical source that is derived from another abstract logical source by defining fields with data from said abstract logical source." ;
                rdfs:subClassOf rml:AbstractLogicalSource ;
                rdfs:isDefinedBy <http://w3id.org/rml/lv/> .


###  http://w3id.org/rml/LogicalViewJoin
rml:LogicalViewJoin rdf:type owl:Class ;
                    rdfs:label "Logical View Join" ;
                    rdfs:comment "A logical view join is an operation that adapts the logical iterations of one logical view (the child logical view) with fields from another logical view (the parent logical view)." ;
                    rdfs:isDefinedBy <http://w3id.org/rml/lv/> .


###  http://w3id.org/rml/ForeignKeyAnnotation
rml:ForeignKeyAnnotation rdf:type owl:Class ;
                      rdfs:label "Foreign Key Annotation" ;
                      rdfs:comment "A foreign key annotation is analogous to the notion of foreign key constraint in databases." ;
                      rdfs:subClassOf rml:InclusionDependencyAnnotation ;
                      rdfs:isDefinedBy <http://w3id.org/rml/lv/> .


###  http://w3id.org/rml/IRISafeAnnotation
rml:IRISafeAnnotation rdf:type owl:Class ;
                   rdfs:label "IRI Safe Annotation" ;
                   rdfs:comment "A IRI safe annotation indicates that the field content is IRI safe." ;
                   rdfs:subClassOf rml:StructuralAnnotation ;
                   rdfs:isDefinedBy <http://w3id.org/rml/lv/> .


###  http://w3id.org/rml/InclusionDependencyAnnotation
rml:InclusionDependencyAnnotation rdf:type owl:Class ;
                               rdfs:label "Inclusion Dependency Annotation" ;
                               rdfs:comment "An inclusion dependency annotation is analogous to the notion of inclusion dependency in databases." ;
                               rdfs:subClassOf rml:StructuralAnnotation ;
                               rdfs:isDefinedBy <http://w3id.org/rml/lv/> .


###  http://w3id.org/rml/NonNullableAnnotation
rml:NonNullableAnnotation rdf:type owl:Class ;
                       rdfs:label "Non Nullable Annotation" ;
                       rdfs:comment "A non nullable annotation is analogous to the notion of NOT NULL constraints in databases." ;
                       rdfs:subClassOf rml:StructuralAnnotation ;
                       rdfs:isDefinedBy <http://w3id.org/rml/lv/> .


###  http://w3id.org/rml/PrimaryKeyAnnotation
rml:PrimaryKeyAnnotation rdf:type owl:Class ;
                      rdfs:label "Primary Key Annotation" ;
                      rdfs:comment "A primary key annotation is analogous to the notion of a primary key constraints in databases." ;
                      rdfs:subClassOf rml:NonNullableAnnotation ,
                                      rml:UniqueAnnotation ;
                      rdfs:isDefinedBy <http://w3id.org/rml/lv/> .


###  http://w3id.org/rml/StructuralAnnotation
rml:StructuralAnnotation rdf:type owl:Class ;
                      rdfs:label "Structural Annotation" ;
                      rdfs:comment "A structural annotation provide a mechanism to express relationships between logical views, as well as additional information about fields." ;
                      rdfs:isDefinedBy <http://w3id.org/rml/lv/> .


###  http://w3id.org/rml/UniqueAnnotation
rml:UniqueAnnotation rdf:type owl:Class ;
                  rdfs:label "Unique Annotation" ;
                  rdfs:comment "A unique annotation is analogous to the notion of UNIQUE constraints in databases. ." ;
                  rdfs:subClassOf rml:StructuralAnnotation ;
                  rdfs:isDefinedBy <http://w3id.org/rml/lv/> .


###  http://www.w3.org/1999/02/22-rdf-syntax-ns#List
rdf:List rdf:type owl:Class .
